

- 1
- (a) $A \cup B \cup C$, At least one of A, B, C occurs,
- (b) $[(A \cap B) \cup (B \cap C) \cup (A \cap C)]^c$, At most one of the events occurs
- (c) $A \cap B \cap C$, A, B, C all occur
- (d) $(A \cap B^c \cap C^c) \cup (A^c \cap B \cap C^c) \cup (A^c \cap B^c \cap C)$, exactly one of A, B, C occurs

2

(a) $A \cup B = A \cup (B \cap A^c)$

Since A & $(B \cap A^c)$ are disjoint, we can apply axiom of probability # 3.

$$P(A \cup B) = P(A) + P(B \cap A^c) \quad \text{--- ①}$$

Next, $B = (B \cap A) \cup (B \cap A^c)$

now again applying probability axiom on disjoint parts,

$$P(B) = P(B \cap A) + P(B \cap A^c)$$

$$\therefore P(B \cap A) = P(B) - P(B \cap A^c) \quad \text{--- ②}$$

$$P(B \cap A^c) = P(B) - P(A \cap B) \quad \text{--- ③}$$

③ in ①,

$$P(A \cup B) = P(A) + [P(B) - P(A \cap B)]$$

$$\therefore P(A \cup B) = P(A) + P(B) - P(A \cap B) \quad \text{--- ④} \quad \text{Q.E.D.}$$

2 (b) To show $P(A) = 1, P(B) = 1 \therefore P(A \cap B) = 1$.

$$P(A \cap B) = P(A) + P(B) - P(A \cup B) \quad \text{from eqn ④ in 2(a)}$$

by substitution we get,

$$P(A \cap B) = 1 + 1 - P(A \cup B) \\ = 2 - P(A \cup B)$$

Since $P(A \cup B) = 1$

$$\therefore P(A \cap B) = 2 - 1 = 1 \quad [\text{Answer}]$$

2. (c) Exactly one of A or B $\Rightarrow (A \cap B^c) \cup (B \cap A^c)$

$$\therefore P(\text{exactly one of A or B}) = P(A \cap B^c) + P(B \cap A^c) \quad \text{Since } A \cap B^c \text{ \& } B \cap A^c \text{ are disjoint}$$

Also,

$$P(A \cap B^c) = P(A) - P(A \cap B)$$

$$P(B \cap A^c) = P(B) - P(A \cap B)$$

Since $A = (A \cap B) \cup (A \cap B^c)$ & union is disjoint

$B = (B \cap A) \cup (B \cap A^c)$ & " " " " from 2(a)

adding them,

$$\therefore P(A \cap B^c) + P(B \cap A^c)$$

$$= (P(A) - P(A \cap B)) + (P(B) - P(A \cap B))$$

$$= P(A) + P(B) - 2P(A \cap B) \quad \text{QED.}$$

2. (d) if $B = (B \cap A) \cup (B \cap A^c)$ shown earlier.

Given $A \subset B \quad \therefore A \cap B = A$

because ^{every} element of A is also an element of B.

$$\therefore A \subset B \Rightarrow A \cap B = A$$

$$\therefore B = A \cup (A^c \cap B)$$

$$\therefore P(B) = P(A) + P(A^c \cap B) \text{ and since } P(A^c \cap B) \geq 0$$

$$\Rightarrow P(B) \geq P(A) \quad \text{Q.E.D.}$$

3. To prove

$$P(A \cup B \cup C) = P(\underbrace{A}) + P(\underbrace{B}) + P(\underbrace{C}) - P(A \cap B) - P(A \cap C) - P(B \cap C) + P(A \cap B \cap C).$$

$$\text{We know } P(\underline{X \cup Y}) = P(X) + P(Y) - P(X \cap Y).$$

$$\therefore P(A \cup B \cup C) = P(A \cup (B \cup C))$$

$$= P(A) + P(\underline{B \cup C}) - P(A \cap (B \cup C))$$

$$= P(A) + P(B) + P(C) - P(B \cap C) - P(A \cap (B \cup C))$$

$$= P(A) + P(B) + P(C) - P(B \cap C) - P((A \cap B) \cup (A \cap C))$$

$$= P(A) + P(B) + P(C) - P(B \cap C) - [P(A \cap B) + P(A \cap C) - P((A \cap B) \cap (A \cap C))]$$

$$= P(A) + P(B) + P(C) - P(B \cap C) - P(A \cap B) - P(A \cap C) + P(A \cap B \cap C)$$

Q.E.D

5. To prove

$$P(A \cap B \cap C) = P(A|B \cap C) P(B|C) P(C)$$

$$P(A|B) = \frac{P(A \cap B)}{P(B)}, \quad P(B) > 0 \quad \text{from conditional prob defn.}$$

$$\therefore P(A|B) P(B) = P(A \cap B)$$

Proof $P(A \cap (B \cap C))$

$$= P(A | B \cap C) P(B \cap C)$$

$$= P(A | B \cap C) P(B | C) P(C)$$

Q.E.D

n.B

$$P(B|C) = \frac{P(B \cap C)}{P(C)}$$

$$\therefore P(B|C) \cdot P(C)$$

$$= P(B \cap C)$$

6.

(a) To show if A & B are independent, then A^c & B are also independent

Here we need to show $P(A^c \cap B) = P(A^c) \cdot P(B)$
expressing B as disjoint union.

$$B = (A \cap B) \cup (A^c \cap B)$$

$$\therefore P(B) = P(A \cap B) + P(A^c \cap B)$$

Since A & B are independent, $P(A \cap B) = P(A) \cdot P(B)$

$$\therefore P(B) = P(A) P(B) + P(A^c \cap B)$$

$$\therefore P(A^c \cap B) = P(B) - P(A) \cdot P(B)$$

$$= P(B) [1 - P(A)]$$

$$= P(B) \cdot P(A^c)$$

hence A^c & B are independent
Q.E.D.

6. (b) Mutually exclusive $\Rightarrow A \cap B = \emptyset$ i.e. disjoint $\therefore P(A \cap B) = 0$

& independent $\Rightarrow P(A \cap B) = P(A) \cdot P(B)$ — (1)

if A & B are both independent & mutually exclusive,
then they must satisfy $P(A) \cdot P(B) = P(A \cap B) = 0$

which requires $P(A) = 0$ or $P(B) = 0$ or both are zero. (5)

So, independent doesn't generally mutually exclusive unless one of the events have zero probability.

if $P(A) > 0$ & $P(B) > 0$, independence & mutually exclusive cannot happen at the same time.

6(c) to show,
if $P(A|B) > P(A)$ then $P(B|A) > P(B)$.

From definition of conditional probability,

$$P(A|B) = \frac{P(A \cap B)}{P(B)} > P(A)$$

multiply both sides by $P(B) > 0$

$$P(A \cap B) > P(A) P(B) \quad \text{--- (1)}$$

$$P(B|A) = \frac{P(B \cap A)}{P(A)}$$

divide each side by $P(A) > 0$ on eqn (1)

$$\frac{P(A \cap B)}{P(A)} > P(B)$$

$$\therefore P(B|A) > P(B)$$

$$\therefore P(A|B) > P(A) \Rightarrow P(B|A) > P(B) \quad \text{Q.E.D.}$$

(7) We need to show

$$P(A \cap B) = P(A) P(B)$$

Using total prob formula

$$P(B) = P(B|A) \cdot P(A) + P(B|A^c) P(A^c)$$

□ □

(8).



$$P(T_S \leq t \mid \text{Server 1}) = \begin{cases} 0 & t \leq 1 \\ \frac{t-1}{4} & 1 < t \leq 5 \\ 1 & t > 5 \end{cases}$$

$$P(T_S \leq t \mid \text{Server 2}) = \begin{cases} 0 & t \leq 1 \\ \frac{t-1}{9} & 1 < t \leq 10 \\ 1 & t > 10 \end{cases}$$

$$P(\{\text{Server 1}\}) = 0.4 \quad \& \quad P(\{\text{Server 2}\}) = 0.6$$

8
(a) To find $P(\{T_S \leq 5\})$

$$\text{Total probability } P(T_S \leq 5) = P(T_S \leq 5 \mid S_1) P(S_1) + P(T_S \leq 5 \mid S_2) P(S_2)$$

$$= \left(\frac{t-1}{4} \right) (0.4) + \left(\frac{t-1}{9} \right) (0.6)$$

$$= \left(\frac{5-1}{4} \right) 0.4 + \left(\frac{5-1}{9} \right) (0.6)$$

$$= 0.4 + \frac{4}{9} \cdot 0.6 = \frac{4}{10} + \frac{24}{90} = \frac{36+24}{90} = \frac{60}{90} = \frac{2}{3}$$

8
(b) $P(\{S_1\} \mid \{T_S \leq 5\}) = \frac{P(T_S \leq 5 \mid S_1) P(S_1)}{P(T_S \leq 5)}$ Bay's Theorem

$$= \frac{1 \cdot 0.4}{(2/3)} = \frac{3}{2} \cdot \frac{4}{10} = \frac{3}{5}$$

8
(c). To find $a > 1$ s.t. $P(\{S_1\} \mid \{T_S \leq a\}) = P(\{S_2\} \mid \{T_S \leq a\})$

$$P(S_1 \mid T_S \leq a) = \left(\frac{a-1}{4} \cdot 0.4 \right) / P(T_S \leq a) = \frac{a-1}{10} \cdot \frac{1}{P(T_S \leq a)}$$

$$P(S_2 \mid T_S \leq a) = \left(\frac{a-1}{9} \cdot 0.6 \right) / P(T_S \leq a) = \frac{a-1}{15} \cdot \frac{1}{P(T_S \leq a)}$$

$$\therefore \frac{a-1}{10} = \frac{a-1}{15} \quad \text{no solution}$$

8

Q75

$$P(s_1 | T_s \leq a) = P(s_2 | T_s \leq a)$$

$$1.0 \cdot 4 = \frac{a-1}{9} \cdot 0.6$$

$$\frac{4}{10} = \frac{a-1}{9} \cdot \frac{6}{10}$$

$$\frac{36}{6} = a-1 \quad \therefore 7 = a \quad \text{answer}$$

④ if $P(A_i) = 1 \forall i \geq 1$ then to show, $P\left(\bigcap_{i=1}^{\infty} A_i\right) = 1$.

From De Morgan's law, $\left(\bigcap_{i=1}^{\infty} A_i\right)^c = \bigcup_{i=1}^{\infty} A_i^c$

we can show prob of complement is zero. i.e. $P\left(\bigcup_{i=1}^{\infty} A_i^c\right) = 0$

$$\text{Since } P(A_i^c) = 1 - P(A_i) = 1 - 1 = 0$$

$$\text{Also } 0 \leq P\left(\bigcup_{i=1}^{\infty} A_i^c\right) \leq \sum_{i=1}^{\infty} P(A_i^c)$$

$$\text{Since } P(A_i^c) = 0 \rightarrow \sum_{i=1}^{\infty} 0 = 0$$

$$\therefore 0 \leq P\left(\bigcup_{i=1}^{\infty} A_i^c\right) \leq 0 \Rightarrow P\left(\bigcup_{i=1}^{\infty} A_i^c\right) = 0$$

$$\begin{aligned} \therefore P\left(\bigcap_{i=1}^{\infty} A_i\right) &= 1 - P\left(\bigcup_{i=1}^{\infty} A_i^c\right) \\ &= 1 - 0 = 1 \end{aligned}$$

$$\therefore P\left(\bigcap_{i=1}^{\infty} A_i\right) = 1.$$

□

⑨ $C \rightarrow$ 'initial choice' of room have car event

$W_s \rightarrow$ event of winning by the switch.

$E \rightarrow$ event that 'initial choice' is empty

$W_{ns} \rightarrow$ event of winning by not switching

Given $P(C) = \frac{1}{3}$ equally probable

$$P(E) = \frac{2}{3}$$

Using TPL we get

$$P(W_s) = P(W_s|C)P(C) + P(W_s|E)P(E)$$

we can consider two conditions. One where contestant switches the door and one where he doesn't

if switches $\Rightarrow P(W_s) =$

if first choice was correct event C , a switch will move away from winning car $\therefore P(W_s|C) = 0$

if first choice is incorrect, (event E) empty door is chosen and host reveals another empty door & unopened door will have car

$$P(W_s|E) = 1$$

$$P(W_s) = 0 \cdot \frac{1}{3} + 1 \cdot \frac{2}{3} = \frac{2}{3}$$

if do not switch,

if first choice is correct & keeps car

$$P(W_{ns}|C) = 1$$

if first choice is incorrect, \rightarrow no car winnings

$$\text{so } P(W_{ns}|E) = 0$$

$$\therefore \cancel{P(W)} P(W_{ns}) = 1 \cdot \frac{1}{3} + 0 \cdot \left(\frac{2}{3}\right) = \frac{1}{3}$$

(11)

$$\therefore P(\text{Switch}) = \frac{2}{3} \quad \& \quad P(\text{not switch}) = \frac{1}{3}$$

\therefore Switching door doubles probability.

— x —